[sledge sem] Fix trans. invariant for llair expressions
Summary:
If the LLVM to llair translation keeps a mapping from register r to
expression e, then for each register r' mentioned in e, there must be an
assignment to r' that dominates the entire live range of r. Thus, where
ever r might be replaced by e, the value of r' will be the same as it
was when the initial assignment to r occurred. Maintaining this
invariant relies on the LLVM being in SSA form.

Reviewed By: jberdine

Differential Revision: D17710288

fbshipit-source-id: fd3eaa57d

sledge/semantics/llvmScript.sml
@@ -145,6 +145,7 @@ Definition terminator_def:
   (terminator (Invoke _ _ _ _ _ _) ⇔ T) ∧
   (terminator Unreachable ⇔ T) ∧
   (terminator Exit ⇔ T) ∧
+  (terminator (Cxa_throw _ _ _) ⇔ T) ∧
   (terminator _ ⇔ F)
 End
 
